Phi_Semantics/PhiSem_Aggregate_Named_Tuple.thy
@@ -57,11 +57,11 @@ debt_axiomatization
             \<open>V_named_tup.mk f1 ## V_named_tup.mk f2 \<longleftrightarrow> (fmdom f1 |\<inter>| fmdom f2 = {||})\<close>
   and   V_named_tup_mult:
             \<open>V_named_tup.mk f1 * V_named_tup.mk f2 = V_named_tup.mk (f1 ++\<^sub>f f2)\<close>
-  and   idx_step_type_tup [eval_semantic_index]:
+  and   idx_step_type_tup [eval_aggregate_path]:
             \<open>s |\<in>| fmdom Ts \<Longrightarrow> idx_step_type (AgIdx_S s) (named_tup.mk Ts) = the (fmlookup Ts s)\<close>
-  and   valid_idx_step_tup[eval_semantic_index]:
+  and   valid_idx_step_tup[eval_aggregate_path]:
             \<open>valid_idx_step (named_tup.mk Ts) j \<longleftrightarrow> j \<in> {AgIdx_S s | s. s |\<in>| fmdom Ts }\<close>
-  and   idx_step_value_named_tup[eval_semantic_index]:
+  and   idx_step_value_named_tup[eval_aggregate_path]:
             \<open>idx_step_value (AgIdx_S s) (V_named_tup.mk vs) = the (fmlookup vs s)\<close>
   and   idx_step_mod_value_named_tup:
             \<open>idx_step_mod_value (AgIdx_S s) f (V_named_tup.mk vs) = V_named_tup.mk (fmupd s (f (the (fmlookup vs s))) vs)\<close>
@@ -112,8 +112,7 @@ translations
 parse_translation \<open>[
   (\<^syntax_const>\<open>\<phi>_named_tuple_\<close>, fn ctxt => fn [sym,T] =>
       Const(\<^const_name>\<open>Named_Tuple_Field\<close>, dummyT)
-          $ (case sym of (Const(\<^syntax_const>\<open>_LOG_EXPR_SYMBOL_\<close>, _) $ x) => x
-                       | _ => Const(\<^const_name>\<open>mk_symbol\<close>, dummyT) $ sym)
+          $ sym
           $ T)
 ]\<close>
 
@@ -128,16 +127,16 @@ print_translation \<open>[
 ]\<close>
 
 lemma Named_Tuple_Field_expn[\<phi>expns]:
-  \<open>p \<in> (x \<Ztypecolon> \<lbrace> LOGIC(s): T \<rbrace>) \<longleftrightarrow> (\<exists>v. p = V_named_tup.mk (fmupd s v fmempty) \<and> v \<in> (x \<Ztypecolon> T))\<close>
+  \<open>p \<in> (x \<Ztypecolon> \<lbrace> LOGIC_SYMBOL(s): T \<rbrace>) \<longleftrightarrow> (\<exists>v. p = V_named_tup.mk (fmupd s v fmempty) \<and> v \<in> (x \<Ztypecolon> T))\<close>
   unfolding Named_Tuple_Field_def \<phi>Type_def by simp
 
 lemma Named_Tuple_Field_inhabited[elim!,\<phi>inhabitance_rule]:
-  \<open>Inhabited (x \<Ztypecolon> \<lbrace> LOGIC(s): T \<rbrace>) \<Longrightarrow> (Inhabited (x \<Ztypecolon> T) \<Longrightarrow> C) \<Longrightarrow> C\<close>
+  \<open>Inhabited (x \<Ztypecolon> \<lbrace> LOGIC_SYMBOL(s): T \<rbrace>) \<Longrightarrow> (Inhabited (x \<Ztypecolon> T) \<Longrightarrow> C) \<Longrightarrow> C\<close>
   unfolding Inhabited_def by (simp add: \<phi>expns)
 
 lemma Empty_Tuple_reduce[simp]:
-  \<open>(((),a) \<Ztypecolon> Empty_Named_Tuple \<^emph> \<lbrace> LOGIC(s): T \<rbrace>) = (a \<Ztypecolon> \<lbrace> LOGIC(s): T \<rbrace>)\<close>
-  \<open>((a,()) \<Ztypecolon> \<lbrace> LOGIC(s): T \<rbrace> \<^emph> Empty_Named_Tuple) = (a \<Ztypecolon> \<lbrace> LOGIC(s): T \<rbrace>)\<close>
+  \<open>(((),a) \<Ztypecolon> Empty_Named_Tuple \<^emph> \<lbrace> LOGIC_SYMBOL(s): T \<rbrace>) = (a \<Ztypecolon> \<lbrace> LOGIC_SYMBOL(s): T \<rbrace>)\<close>
+  \<open>((a,()) \<Ztypecolon> \<lbrace> LOGIC_SYMBOL(s): T \<rbrace> \<^emph> Empty_Named_Tuple) = (a \<Ztypecolon> \<lbrace> LOGIC_SYMBOL(s): T \<rbrace>)\<close>
   unfolding set_eq_iff
   by ((clarsimp; rule; clarsimp simp add: \<phi>expns V_named_tup_mult V_named_tup_sep_disj),
       blast,
@@ -148,7 +147,7 @@ lemma Empty_Tuple_reduce[simp]:
 
 
 lemma Named_Tuple_Field_zero  [\<phi>reason 1000]:
-  \<open>\<phi>Zero ty T x \<Longrightarrow> \<phi>Zero (named_tup.mk (fmupd s ty fmempty)) \<lbrace> LOGIC(s): T \<rbrace> x \<close>
+  \<open>\<phi>Zero ty T x \<Longrightarrow> \<phi>Zero (named_tup.mk (fmupd s ty fmempty)) \<lbrace> LOGIC_SYMBOL(s): T \<rbrace> x \<close>
   unfolding \<phi>Zero_def
   by (clarsimp simp add: \<phi>expns,
       metis (mono_tags, lifting) Named_Tuple_Field_expn comp_apply fmmap_empty fmmap_fmupd fmpred_empty fmpred_upd image_eqI option.sel)
@@ -157,7 +156,7 @@ lemma Tuple_Field_zeros [\<phi>reason 1000]:
   \<open> s |\<notin>| fmdom tys
 \<Longrightarrow> \<phi>Zero ty T x
 \<Longrightarrow> \<phi>Zero (named_tup.mk tys) Ts xs
-\<Longrightarrow> \<phi>Zero (named_tup.mk (fmupd s ty tys)) (\<lbrace> LOGIC(s): T \<rbrace> \<^emph> Ts) (x,xs) \<close>
+\<Longrightarrow> \<phi>Zero (named_tup.mk (fmupd s ty tys)) (\<lbrace> LOGIC_SYMBOL(s): T \<rbrace> \<^emph> Ts) (x,xs) \<close>
   unfolding \<phi>Zero_def
   apply (clarsimp simp add: \<phi>expns; cases \<open>fmpred (\<lambda>_ t. \<exists>y. Zero t = Some y) tys\<close>;
      auto simp add: inj_image_mem_iff \<phi>expns fmmap_fmupd
@@ -169,46 +168,46 @@ lemma Tuple_Field_zeros [\<phi>reason 1000]:
 
 lemma Tuple_Field_semty[\<phi>reason 1000]:
   \<open> \<phi>SemType (x \<Ztypecolon> T) TY
-\<Longrightarrow> \<phi>SemType (x \<Ztypecolon> \<lbrace> LOGIC(s): T \<rbrace>) (named_tup.mk (fmupd s TY fmempty))\<close>
+\<Longrightarrow> \<phi>SemType (x \<Ztypecolon> \<lbrace> LOGIC_SYMBOL(s): T \<rbrace>) (named_tup.mk (fmupd s TY fmempty))\<close>
   unfolding \<phi>SemType_def subset_iff
   by (clarsimp simp add: \<phi>expns; blast)
 
 lemma Tuple_Field_semtys[\<phi>reason 1000]:
   \<open> \<phi>SemType (x \<Ztypecolon> T) TY
 \<Longrightarrow> \<phi>SemType (xs \<Ztypecolon> Ts) (named_tup.mk TYs)
-\<Longrightarrow> \<phi>SemType ((x,xs) \<Ztypecolon> (\<lbrace> LOGIC(s): T \<rbrace> \<^emph> Ts)) (named_tup.mk (fmupd s TY TYs))\<close>
+\<Longrightarrow> \<phi>SemType ((x,xs) \<Ztypecolon> (\<lbrace> LOGIC_SYMBOL(s): T \<rbrace> \<^emph> Ts)) (named_tup.mk (fmupd s TY TYs))\<close>
   unfolding \<phi>SemType_def subset_iff
   by (clarsimp simp add: \<phi>expns; metis V_named_tup_mult fmadd_empty(2) fmadd_fmupd fmrel_upd)
 
 subsection \<open>Index\<close>
 
 lemma [\<phi>reason 1200]:
-  \<open> \<g>\<u>\<a>\<r>\<d> s' \<noteq> s
+  \<open> \<g>\<u>\<a>\<r>\<d> \<c>\<o>\<n>\<d>\<i>\<t>\<i>\<o>\<n> s' \<noteq> s
 \<Longrightarrow> \<phi>Index_getter (AgIdx_S s' # idx) X Y f
-\<Longrightarrow> \<phi>Index_getter (AgIdx_S s' # idx) (\<lbrace> LOGIC(s): T \<rbrace> \<^emph> X) Y (f o snd)\<close>
+\<Longrightarrow> \<phi>Index_getter (AgIdx_S s' # idx) (\<lbrace> LOGIC_SYMBOL(s): T \<rbrace> \<^emph> X) Y (f o snd)\<close>
   unfolding \<phi>Index_getter_def
   by (clarsimp simp add: \<phi>expns,
       metis V_named_tup_mult V_named_tup_sep_disj_L fmadd_empty(2) fmadd_fmupd fmupd_lookup idx_step_value_named_tup)
 
 lemma [\<phi>reason 1201]:
-  \<open> \<g>\<u>\<a>\<r>\<d> s' = s
+  \<open> \<g>\<u>\<a>\<r>\<d> \<c>\<o>\<n>\<d>\<i>\<t>\<i>\<o>\<n> s' = s
 \<Longrightarrow> \<phi>Index_getter idx T Y f
-\<Longrightarrow> \<phi>Index_getter (AgIdx_S s' # idx) (\<lbrace> LOGIC(s): T \<rbrace> \<^emph> X) Y (f o fst)\<close>
+\<Longrightarrow> \<phi>Index_getter (AgIdx_S s' # idx) (\<lbrace> LOGIC_SYMBOL(s): T \<rbrace> \<^emph> X) Y (f o fst)\<close>
   unfolding \<phi>Index_getter_def
   by (clarsimp simp add: \<phi>expns,
       metis V_named_tup_mult V_named_tup_sep_disj_L fmadd_fmupd fmupd_lookup idx_step_value_named_tup option.sel)
 
 lemma [\<phi>reason 1201]:
-  \<open> \<g>\<u>\<a>\<r>\<d> s' = s
+  \<open> \<g>\<u>\<a>\<r>\<d> \<c>\<o>\<n>\<d>\<i>\<t>\<i>\<o>\<n> s' = s
 \<Longrightarrow> \<phi>Index_getter idx T Y f
-\<Longrightarrow> \<phi>Index_getter (AgIdx_S s' # idx) \<lbrace> LOGIC(s): T \<rbrace> Y f\<close>
+\<Longrightarrow> \<phi>Index_getter (AgIdx_S s' # idx) \<lbrace> LOGIC_SYMBOL(s): T \<rbrace> Y f\<close>
   unfolding \<phi>Index_getter_def
   by (clarsimp simp add: \<phi>expns, metis fmupd_lookup idx_step_value_named_tup option.sel)
 
 lemma [\<phi>reason 1200]:
-  \<open> \<g>\<u>\<a>\<r>\<d> s' \<noteq> s
+  \<open> \<g>\<u>\<a>\<r>\<d> \<c>\<o>\<n>\<d>\<i>\<t>\<i>\<o>\<n> s' \<noteq> s
 \<Longrightarrow> \<phi>Index_mapper (AgIdx_S s' # idx) X X' Y Y' f
-\<Longrightarrow> \<phi>Index_mapper (AgIdx_S s' # idx) (\<lbrace> LOGIC(s): T \<rbrace> \<^emph> X) (\<lbrace> LOGIC(s): T \<rbrace> \<^emph> X') Y Y' (apsnd o f)\<close>
+\<Longrightarrow> \<phi>Index_mapper (AgIdx_S s' # idx) (\<lbrace> LOGIC_SYMBOL(s): T \<rbrace> \<^emph> X) (\<lbrace> LOGIC_SYMBOL(s): T \<rbrace> \<^emph> X') Y Y' (apsnd o f)\<close>
   unfolding \<phi>Index_mapper_def
   apply (clarsimp simp add: \<phi>expns )
   subgoal premises prems for g g' a b c' v' proof -
@@ -223,9 +222,9 @@ lemma [\<phi>reason 1200]:
   qed .
 
 lemma [\<phi>reason 1201]:
-  \<open> \<g>\<u>\<a>\<r>\<d> s' = s
+  \<open> \<g>\<u>\<a>\<r>\<d> \<c>\<o>\<n>\<d>\<i>\<t>\<i>\<o>\<n> s' = s
 \<Longrightarrow> \<phi>Index_mapper idx X X' Y Y' f
-\<Longrightarrow> \<phi>Index_mapper (AgIdx_S s' # idx) (\<lbrace> LOGIC(s): X \<rbrace> \<^emph> R) (\<lbrace> LOGIC(s): X' \<rbrace> \<^emph> R) Y Y' (apfst o f)\<close>
+\<Longrightarrow> \<phi>Index_mapper (AgIdx_S s' # idx) (\<lbrace> LOGIC_SYMBOL(s): X \<rbrace> \<^emph> R) (\<lbrace> LOGIC_SYMBOL(s): X' \<rbrace> \<^emph> R) Y Y' (apfst o f)\<close>
   unfolding \<phi>Index_mapper_def
   apply (clarsimp simp add: \<phi>expns )
   subgoal premises prems for g g' a b c' v' proof -
@@ -236,9 +235,9 @@ lemma [\<phi>reason 1201]:
   qed .
 
 lemma [\<phi>reason 1201]:
-  \<open> \<g>\<u>\<a>\<r>\<d> s' = s
+  \<open> \<g>\<u>\<a>\<r>\<d> \<c>\<o>\<n>\<d>\<i>\<t>\<i>\<o>\<n> s' = s
 \<Longrightarrow> \<phi>Index_mapper idx X X' Y Y' f
-\<Longrightarrow> \<phi>Index_mapper (AgIdx_S s' # idx) \<lbrace> LOGIC(s): X \<rbrace> \<lbrace> LOGIC(s): X' \<rbrace> Y Y' f\<close>
+\<Longrightarrow> \<phi>Index_mapper (AgIdx_S s' # idx) \<lbrace> LOGIC_SYMBOL(s): X \<rbrace> \<lbrace> LOGIC_SYMBOL(s): X' \<rbrace> Y Y' f\<close>
   unfolding \<phi>Index_mapper_def
   by (clarsimp simp add: \<phi>expns, metis fmupd_idem fmupd_lookup idx_step_mod_value_named_tup option.sel)
 
