Phi_Semantics/PhiSem_Aggregate_Path.thy
@@ -15,29 +15,52 @@ syntax "_ID_ag_idx_"  :: \<open>\<phi>_symbol_ \<Rightarrow> \<phi>_ag_idx_\<clo
        "_0_ag_idx_"   :: \<open>\<phi>_ag_idx_\<close> ("0")
        "_1_ag_idx_"   :: \<open>\<phi>_ag_idx_\<close> ("1")
        "_num_ag_idx_" :: \<open>num_token \<Rightarrow> \<phi>_ag_idx_\<close> ("_")
-       "_log_ag_idx_" :: \<open>logic \<Rightarrow> \<phi>_ag_idx_\<close> ("LOGIC'(_')")
-       "_MK_ag_idx_"  :: \<open>\<phi>_ag_idx_ \<Rightarrow> aggregate_index\<close> ("\<phi>AG'_IDX'(_')")
+       "_log_ag_idx_" :: \<open>logic \<Rightarrow> \<phi>_ag_idx_\<close> ("LOGIC'_IDX'(_')")
+       "_log_num_ag_idx_" :: \<open>logic \<Rightarrow> \<phi>_ag_idx_\<close> ("_\<^sup>\<t>\<^sup>\<h>" [1000] 999)
+       "_log_num_ag_idx'_" :: \<open>logic \<Rightarrow> \<phi>_ag_idx_\<close> ("'(_')\<^sup>\<t>\<^sup>\<h>")
+       "_log_num_ag_idx_ascii_" :: \<open>logic \<Rightarrow> \<phi>_ag_idx_\<close> ("#_" [1000] 999)
+       "_log_num_ag_idx_ascii'_" :: \<open>logic \<Rightarrow> \<phi>_ag_idx_\<close> ("#'(_')")
+       "_MK_ag_idx_"  :: \<open>\<phi>_ag_idx_ \<Rightarrow> aggregate_index\<close> ("AG'_IDX'(_')")
 
 ML \<open>
 structure Phi_Aggregate_Syntax = struct
 
 fun parse_index (Const(\<^syntax_const>\<open>_ID_ag_idx_\<close> , _) $ id) =
-        Const(\<^const_name>\<open>AgIdx_S\<close>, dummyT) $ (Const(\<^const_name>\<open>mk_symbol\<close>, dummyT) $ id)
+        Const(\<^const_name>\<open>AgIdx_S\<close>, dummyT) $ id
   | parse_index (Const(\<^syntax_const>\<open>_num_ag_idx_\<close>, _) $ Free (n, _)) =
         Const(\<^const_name>\<open>AgIdx_N\<close>, dummyT) $ mk_numeral_nat (Value.parse_nat n)
   | parse_index (Const(\<^syntax_const>\<open>_log_ag_idx_\<close>, _) $ tm) = tm
+  | parse_index (Const(\<^syntax_const>\<open>_log_num_ag_idx_\<close>, _) $ tm) =
+        Const(\<^const_name>\<open>AgIdx_N\<close>, dummyT) $ tm
+  | parse_index (Const(\<^syntax_const>\<open>_log_num_ag_idx'_\<close>, _) $ tm) =
+        Const(\<^const_name>\<open>AgIdx_N\<close>, dummyT) $ tm
+  | parse_index (Const(\<^syntax_const>\<open>_log_num_ag_idx_ascii_\<close>, _) $ tm) =
+        Const(\<^const_name>\<open>AgIdx_N\<close>, dummyT) $ tm
+  | parse_index (Const(\<^syntax_const>\<open>_log_num_ag_idx_ascii'_\<close>, _) $ tm) =
+        Const(\<^const_name>\<open>AgIdx_N\<close>, dummyT) $ tm
   | parse_index (Const(\<^syntax_const>\<open>_0_ag_idx_\<close>, _)) =
         Const(\<^const_name>\<open>AgIdx_N\<close>, dummyT) $ mk_numeral_nat 0
   | parse_index (Const(\<^syntax_const>\<open>_1_ag_idx_\<close>, _)) =
         Const(\<^const_name>\<open>AgIdx_N\<close>, dummyT) $ mk_numeral_nat 1
   | parse_index x = (@{print} x; error "SYNTAX ERROR #ee2e77a2-b6d7-4acf-ae18-5d266dc2f06e")
 
+fun is_atom (Const ("_free", _) $ X) = is_atom X
+  | is_atom (Const ("_var", _) $ X) = is_atom X
+  | is_atom (_ $ _) = false
+  | is_atom _ = true
+
 fun print_index (Const(\<^const_syntax>\<open>AgIdx_S\<close>, _) $ (Const(\<^const_syntax>\<open>mk_symbol\<close>, _) $ tm)) =
      (case Phi_Tool_Symbol.revert_symbol (dest_synt_numeral tm)
         of SOME id => Free(id, dummyT)
          | NONE => tm)
+  | print_index (Const(\<^const_syntax>\<open>AgIdx_S\<close>, _) $ tm) =
+     Const (\<^syntax_const>\<open>_LOG_EXPR_SYMBOL_\<close>, dummyT) $ tm
   | print_index (Const (\<^const_syntax>\<open>AgIdx_N\<close>, _) $ tm) =
-      Free(string_of_int (dest_synt_numeral tm), dummyT)
+      (case try dest_synt_numeral tm
+         of SOME N => Const(\<^syntax_const>\<open>_log_num_ag_idx_\<close>, dummyT) $ Free(string_of_int N, dummyT)
+          | _ => if is_atom tm
+                 then Const(\<^syntax_const>\<open>_log_num_ag_idx_\<close>, dummyT) $ tm
+                 else Const(\<^syntax_const>\<open>_log_num_ag_idx'_\<close>, dummyT) $ tm)
   | print_index tm = Const(\<^syntax_const>\<open>_log_ag_idx_\<close>, dummyT) $ tm
 
 end
@@ -54,10 +77,13 @@ print_translation \<open>[
          | NONE => tm)),
   (\<^const_syntax>\<open>AgIdx_N\<close>, (fn ctxt => fn [tm] =>
       case try dest_synt_numeral tm
-        of SOME N => Const (\<^syntax_const>\<open>_MK_ag_idx_\<close>, dummyT) $ Free(string_of_int N, dummyT)))
+        of SOME N => Const (\<^syntax_const>\<open>_MK_ag_idx_\<close>, dummyT) $
+                        (Const(\<^syntax_const>\<open>_log_num_ag_idx_\<close>, dummyT) $ Free(string_of_int N, dummyT))
+         | NONE => Const (\<^syntax_const>\<open>_MK_ag_idx_\<close>, dummyT) $ (
+            if Phi_Aggregate_Syntax.is_atom tm
+            then Const (\<^syntax_const>\<open>_log_num_ag_idx_\<close>, dummyT) $ tm
+            else Const (\<^syntax_const>\<open>_log_num_ag_idx'_\<close>, dummyT) $ tm)))
 ]\<close>
-
-
 
 
 end
