Phi_Semantics/PhiTool_Symbol.thy
@@ -22,7 +22,7 @@ ML_file \<open>PhiTool_Symbol.ML\<close>
 nonterminal "\<phi>_symbol_"
 
 syntax "_ID_SYMBOL_" :: \<open>id \<Rightarrow> \<phi>_symbol_\<close> ("_")
-       "_LOG_EXPR_SYMBOL_" :: \<open>logic \<Rightarrow> \<phi>_symbol_\<close> ("LOGIC'(_')")
+       "_LOG_EXPR_SYMBOL_" :: \<open>logic \<Rightarrow> \<phi>_symbol_\<close> ("LOGIC'_SYMBOL'(_')")
        "_MK_SYMBOL_" :: \<open>\<phi>_symbol_ \<Rightarrow> symbol\<close> ("SYMBOL'(_')")
 
 declare [[ML_debugger]]
@@ -31,7 +31,7 @@ ML \<open>
 structure Phi_Tool_Symbol = struct
 open Phi_Tool_Symbol
 
-fun parse (Free (id, _)) = Phi_Tool_Symbol.mk_symbol id
+fun parse (Free (id, _)) = Const(\<^const_name>\<open>mk_symbol\<close>, dummyT) $ Phi_Tool_Symbol.mk_symbol id
   | parse tm = (@{print} tm; error "Expect an identifier.")
 
 fun print tm =
@@ -43,12 +43,15 @@ fun print tm =
 end
 \<close>
 
+declare [[ML_debugger]]
+
 parse_translation \<open>[
   (\<^syntax_const>\<open>_ID_SYMBOL_\<close>, (fn ctxt => fn [x] => Phi_Tool_Symbol.parse x)),
-  (\<^syntax_const>\<open>_MK_SYMBOL_\<close>, (fn ctxt =>
-    (fn [Const(\<^syntax_const>\<open>_LOG_EXPR_SYMBOL_\<close>, _) $ x] => x
-      | [x] => Const(\<^const_name>\<open>mk_symbol\<close>, dummyT) $ x)))
+  (\<^syntax_const>\<open>_LOG_EXPR_SYMBOL_\<close>, (fn ctxt => fn [x] =>
+        Const (\<^syntax_const>\<open>_constrain\<close>, dummyT) $ x $ Const(\<^type_syntax>\<open>symbol\<close>, dummyT))),
+  (\<^syntax_const>\<open>_MK_SYMBOL_\<close>, (fn ctxt => fn [x] => x))
 ]\<close>
+
 
 print_translation \<open>[
   (\<^const_syntax>\<open>mk_symbol\<close>, (fn ctxt => fn [tm] => Const (\<^syntax_const>\<open>_MK_SYMBOL_\<close>, dummyT) $ Phi_Tool_Symbol.print tm))
