Phi_System/IDE_CP_Reasoning1.thy
@@ -149,23 +149,23 @@ structure Assertion_SS_Abnormal = Simpset (
 
 \<phi>reasoner_ML assertion_simp_source 1300
   (\<open>Simplify (assertion_simps SOURCE) ?X' ?X\<close>)
-  = \<open>PLPR_Simplifier.simplifier_by_ss' NONE (fn ctxt =>
+  = \<open>PLPR_Simplifier.simplifier_by_ss' (fn ctxt =>
       Raw_Simplifier.merge_ss (Assertion_SS.get' ctxt, Assertion_SS_Source.get' ctxt))\<close>
 
 \<phi>reasoner_ML assertion_simp_target 1300
   (\<open>Simplify (assertion_simps TARGET) ?X' ?X\<close>)
-  = \<open>PLPR_Simplifier.simplifier_by_ss' NONE (fn ctxt =>
+  = \<open>PLPR_Simplifier.simplifier_by_ss' (fn ctxt =>
       Raw_Simplifier.merge_ss (Assertion_SS.get' ctxt, Assertion_SS_Target.get' ctxt))\<close>
 
 \<phi>reasoner_ML assertion_simp_abnormal 1300
   (\<open>Simplify (assertion_simps ABNORMAL) ?X' ?X\<close>)
-  = \<open>PLPR_Simplifier.simplifier_by_ss' NONE (fn ctxt =>
+  = \<open>PLPR_Simplifier.simplifier_by_ss' (fn ctxt =>
       Raw_Simplifier.merge_ss (Assertion_SS.get' ctxt, Assertion_SS_Abnormal.get' ctxt))\<close>
 
 \<phi>reasoner_ML assertion_simp 1200
   (\<open>Premise (assertion_simps _) _\<close> | \<open>Simplify (assertion_simps ?ANY) ?X' ?X\<close>
      )
-  = \<open>PLPR_Simplifier.simplifier_by_ss' NONE Assertion_SS.get'\<close>
+  = \<open>PLPR_Simplifier.simplifier_by_ss' Assertion_SS.get'\<close>
 
 lemmas [assertion_simps] =
   mult_zero_right[where 'a=\<open>'a::sep_magma set\<close>] mult_zero_left[where 'a=\<open>'a::sep_magma set\<close>]
@@ -188,8 +188,14 @@ consts MODE_\<phi>EXPN :: mode \<comment> \<open>relating to named_theorems \<op
 
 abbreviation \<phi>expn_Premise ("<\<phi>expn> _" [26] 26) where \<open>\<phi>expn_Premise \<equiv> Premise MODE_\<phi>EXPN\<close>
 
-\<phi>reasoner \<phi>expn_Premise 10 (\<open><\<phi>expn> ?P\<close>)
-  = (rule Premise_I; simp add: \<phi>expns useful)
+\<phi>reasoner_ML \<phi>expn_Premise 10 (\<open><\<phi>expn> ?P\<close>) = \<open>
+  Seq.ORELSE (
+  PLPR_Simplifier.simplifier (fn ctxt =>
+    ctxt addsimps (Useful_Thms.get ctxt)),
+  PLPR_Simplifier.simplifier (fn ctxt =>
+    ctxt addsimps (Useful_Thms.get ctxt @ Named_Theorems.get ctxt \<^named_theorems>\<open>\<phi>expns\<close>)))
+\<close>
+
 
 text \<open>Antecedent \<^prop>\<open><\<phi>expn> P\<close> indicates the reasoner solving the premise \<^prop>\<open>P\<close> using
   simplification rules of \<open>\<phi>expns\<close>.\<close>
@@ -353,7 +359,7 @@ declare mult.assoc[symmetric, frame_var_rewrs]
 consts frame_var_rewrs :: mode
 
 \<phi>reasoner_ML Subty_Simplify 2000 (\<open>Simplify frame_var_rewrs ?x ?y\<close>)
-  = \<open>PLPR_Simplifier.simplifier_only NONE (fn ctxt =>
+  = \<open>PLPR_Simplifier.simplifier_only (fn ctxt =>
           Named_Theorems.get ctxt \<^named_theorems>\<open>frame_var_rewrs\<close>)\<close>
 
 definition \<phi>IntroFrameVar :: "'a::sep_magma_1 set \<Rightarrow> 'a set \<Rightarrow> 'a set \<Rightarrow> 'a set \<Rightarrow> 'a set \<Rightarrow> bool"
